ETCSsettings.sml
@@ -1,3 +1,7 @@
+fun store_as name th = 
+let val _ = store_thm(name, th)
+in th
+end
 
 local
 fun delete'(set,mem) = HOLset.delete(set,mem) handle _ => set
@@ -85,78 +89,82 @@ fun new_ax f =
     in
         mk_thm(essps,[],f)
     end
+ 
+fun store_ax (name,f) = store_as name (new_ax f)
 
+val idL = store_ax("idL", “!B A f:B->A. id(A) o f = f”);
 
-val idL = new_ax “!B A f:B->A. id(A) o f = f”
+val idR = store_ax("idR",“!A B f:A->B. f o id(A) = f”);
 
-val idR = new_ax “!A B f:A->B. f o id(A) = f”
-
-val o_assoc = new_ax “!A.!B.!f: A -> B.!C.!g:B -> C.!D.!h: C -> D.(h o g) o f = h o g o f”
+val o_assoc = store_ax("o_assoc",“!A.!B.!f: A -> B.!C.!g:B -> C.!D.!h: C -> D.(h o g) o f = h o g o f”);
 
 val _ = new_pred "is1" [("ONE",ob_sort)]
 
-val is1_def = new_ax “!ONE. is1(ONE) <=> !X.?!f:X->ONE.T”
+val is1_def = store_ax("is1_def",“!ONE. is1(ONE) <=> !X.?!f:X->ONE.T”)
 
-val ONE_ex = new_ax “?ONE.is1(ONE)”
+val ONE_ex = store_ax("ONE_ex",“?ONE.is1(ONE)”)
 
 fun ex2fsym0 name args th = th |> eqT_intro |> iffRL |> ex2fsym name args
                                |> C mp (trueI [])
                     
-val ONE_def = ex2fsym0 "1" [] ONE_ex
+val ONE_def = ex2fsym0 "1" [] ONE_ex |> store_as "ONE_def"
 
 val ONE_prop = ONE_def |> rewr_rule [is1_def]
+                       |> store_as "ONE_prop"
+
 (*why rewr_rule with is1_def loops? it thought is1 is fVar notpred  TODO*)
 
-val To1_def = ONE_prop |> spec_all |> uex_expand |> ex2fsym0 "To1" ["X"] |> gen_all
+val To1_def = ONE_prop |> spec_all |> uex_expand |> ex2fsym0 "To1" ["X"] |> gen_all |> store_as "To1_def"
 
 val _ = new_pred "is0" [("ZERO",ob_sort)]
 
-val is0_def = new_ax “!ZERO.is0(ZERO) <=> !X.?!f:ZERO ->X. T”
+val is0_def = store_ax("is0_def",“!ZERO.is0(ZERO) <=> !X.?!f:ZERO ->X. T”)
 
-val ZERO_ex = new_ax “?ZERO.is0(ZERO)”
+val ZERO_ex = store_ax("ZERO_ex",“?ZERO.is0(ZERO)”)
 
-val ZERO_def = ex2fsym0 "0" [] ZERO_ex
+val ZERO_def = ex2fsym0 "0" [] ZERO_ex |> store_as "ZERO_def"
 
-val ZERO_prop = ZERO_def |> conv_rule (once_depth_fconv no_conv (rewr_fconv (spec_all is0_def)))
+val ZERO_prop = ZERO_def |> conv_rule (once_depth_fconv no_conv (rewr_fconv (spec_all is0_def))) |> store_as "ZERO_prop"
 
-val From0_def = ZERO_prop |> spec_all |> uex_expand |> ex2fsym0 "From0" ["X"] |> gen_all
+val From0_def = ZERO_prop |> spec_all |> uex_expand |> ex2fsym0 "From0" ["X"] |> gen_all |> store_as "From0_def"
 
 val _ = new_pred "isPr" [("p1",ar_sort (mk_ob "AB") (mk_ob "A")),
                          ("p2",ar_sort (mk_ob "AB") (mk_ob "B"))]
 
-val isPr_def = new_ax “!A B AB p1:AB->A p2:AB->B. isPr(p1,p2) <=>
-   !X f:X->A g:X->B.?!fg:X->AB. p1 o fg = f & p2 o fg = g”
+val isPr_def = store_ax("isPr_def",“!A B AB p1:AB->A p2:AB->B. isPr(p1,p2) <=>
+   !X f:X->A g:X->B.?!fg:X->AB. p1 o fg = f & p2 o fg = g”)
 
-val isPr_ex = new_ax “!A B.?AB p1:AB->A p2:AB->B.isPr(p1,p2)”;
+val isPr_ex = store_ax("isPr_ex",“!A B.?AB p1:AB->A p2:AB->B.isPr(p1,p2)”);
 
-val Po_def = isPr_ex |> spec_all |> ex2fsym0 "*" ["A","B"] |> gen_all
+val Po_def = isPr_ex |> spec_all |> ex2fsym0 "*" ["A","B"] |> gen_all |> store_as "Po_def"
 
-val p1_def = Po_def |> spec_all |> ex2fsym0 "p1" ["A","B"] |> gen_all
+val p1_def = Po_def |> spec_all |> ex2fsym0 "p1" ["A","B"] |> gen_all |> store_as "p1_def"
 
-val p2_def = p1_def |> spec_all |> ex2fsym0 "p2" ["A","B"] |> gen_all
+val p2_def = p1_def |> spec_all |> ex2fsym0 "p2" ["A","B"] |> gen_all |> store_as "p2_def"
 
 val Pa_def = p2_def |> rewr_rule[isPr_def] |> spec_all
                     |> uex_expand 
                     |> ex2fsym0 "Pa" ["f","g"]
-
+                    |> store_as "Pa_def"
 
 val _ = new_pred "iscoPr" [("i1",ar_sort (mk_ob "A") (mk_ob "AB")),
                            ("i2",ar_sort (mk_ob "B") (mk_ob "AB"))]
 
-val iscoPr_def = new_ax “!A B AB i1:A->AB i2:B->AB. iscoPr(i1,i2) <=>
-   !X f:A->X g:B->X.?!fg:AB->X.fg o i1 = f & fg o i2 = g”
+val iscoPr_def = store_ax("iscoPr_def",“!A B AB i1:A->AB i2:B->AB. iscoPr(i1,i2) <=>
+   !X f:A->X g:B->X.?!fg:AB->X.fg o i1 = f & fg o i2 = g”);
 
-val iscoPr_ex = new_ax “!A B.?AB i1:A->AB i2:B->AB.iscoPr(i1,i2)”;
+val iscoPr_ex = store_ax("iscoPr_ex",“!A B.?AB i1:A->AB i2:B->AB.iscoPr(i1,i2)”);
 
-val coPo_def = iscoPr_ex |> spec_all |> ex2fsym0 "+" ["A","B"] |> gen_all
+val coPo_def = iscoPr_ex |> spec_all |> ex2fsym0 "+" ["A","B"] |> gen_all |> store_as "coPo_def";
 
-val i1_def = coPo_def |> spec_all |> ex2fsym0 "i1" ["A","B"] |> gen_all
+val i1_def = coPo_def |> spec_all |> ex2fsym0 "i1" ["A","B"] |> gen_all |> store_as "i1_def";
 
-val i2_def = i1_def |> spec_all |> ex2fsym0 "i2" ["A","B"] |> gen_all
+val i2_def = i1_def |> spec_all |> ex2fsym0 "i2" ["A","B"] |> gen_all |> store_as "i2_def";
 
 val coPa_def = i2_def |> rewr_rule[iscoPr_def] |> spec_all
                       |> uex_expand 
                       |> ex2fsym0 "coPa" ["f","g"]
+                      |> store_as "coPa_def";
 
 
 (*TODO: if ispr i.e. formula variable, then will loop*)
@@ -164,16 +172,16 @@ val coPa_def = i2_def |> rewr_rule[iscoPr_def] |> spec_all
 val _ = new_pred "isEq" 
                  [("f",ar_sort (mk_ob "A") (mk_ob "B")),
                   ("g",ar_sort (mk_ob "A") (mk_ob "B")),
-                  ("e",ar_sort (mk_ob "E") (mk_ob "A"))]
+                  ("e",ar_sort (mk_ob "E") (mk_ob "A"))];
 
-val isEq_def = new_ax 
+val isEq_def = store_ax("isEq_def",
 “!A B f:A->B g E e:E->A. 
       isEq(f,g,e) <=> 
       f o e = g o e & 
       !X a:X->A. f o a = g o a ==>
-      ?!a0:X->E. a = e o a0”
+      ?!a0:X->E. a = e o a0”)
 
-val isEq_ex = new_ax “!A B f:A->B g:A->B.?E e:E->A.isEq(f,g,e)”
+val isEq_ex = store_ax("isEq_ex",“!A B f:A->B g:A->B.?E e:E->A.isEq(f,g,e)”)
 
 val Eqa_def = 
     isEq_def |> iffLR 
@@ -181,21 +189,21 @@ val Eqa_def =
              |> spec_all |> undisch |> uex_expand
              |> conj_all_assum |> disch_all
              |> ex2fsym "Eqa" ["f","g","e","a"]
-
+             |> store_as "Eqa_def"
 
 val _ = new_pred "iscoEq" 
                  [("f",ar_sort (mk_ob "A") (mk_ob "B")),
                   ("g",ar_sort (mk_ob "A") (mk_ob "B")),
                   ("ce",ar_sort (mk_ob "B") (mk_ob "cE"))]
 
-val iscoEq_def = new_ax 
+val iscoEq_def = store_ax("iscoEq_def",
 “!A B f:A->B g cE ce:B -> cE. 
       iscoEq(f,g,ce) <=> 
       ce o f = ce o g & 
       !X x:B->X. x o f = x o g ==>
-      ?!x0:cE->X. x = x0 o ce”
+      ?!x0:cE->X. x = x0 o ce”)
 
-val iscoEq_ex = new_ax “!A B f:A->B g:A->B.?cE ce:B->cE.iscoEq(f,g,ce)”;
+val iscoEq_ex = store_ax("iscoEq_ex",“!A B f:A->B g:A->B.?cE ce:B->cE.iscoEq(f,g,ce)”);
 
 val coEqa_def = 
     iscoEq_def |> iffLR 
@@ -203,6 +211,7 @@ val coEqa_def =
                |> spec_all |> undisch |> uex_expand
                |> conj_all_assum |> disch_all
                |> ex2fsym "coEqa" ["f","g","ce","x"]
+               |> store_as "coEqa_def"
 (*TodO tidy the conjs to imp here*)
 
 
@@ -218,53 +227,74 @@ h
 BA such that (A × h)e = f. This
 universal mapping property is partly expressed by the following diagram.
 *)
+
 val _ = new_pred "isExp" 
  [("ev",ar_sort (Po (mk_ob "A") (mk_ob "A2B")) (mk_ob "B"))]
 
 val isExp_def =
- new_ax “!A B A2B ev:A * A2B -> B.
-         isExp(ev) <=> !X f:A * X->B. ?!h:X->A2B. ev o Pa(p1(A,X), h o p2(A,X)) = f”
+ store_ax("isExp_def",“!A B A2B ev:A * A2B -> B.
+         isExp(ev) <=> !X f:A * X->B. ?!h:X->A2B. ev o Pa(p1(A,X), h o p2(A,X)) = f”)
 
 
 (*example here : we cannot get function for eqlz, because the inputs are a pair of ars, and we need to produce an object first. But here the input are objects, we can produce an object from the objects first, the exp, and then have ev(A,B)*)
 
-val isExp_ex = new_ax “!A B. ?A2B ev:A * A2B->B. isExp(ev)”
+val isExp_ex = store_ax("isExp_ex",“!A B. ?A2B ev:A * A2B->B. isExp(ev)”)
 
 val Exp_def = isExp_ex |> spec_all 
                        |> ex2fsym0 "Exp" ["A","B"] |> gen_all
+                       |> store_as "Exp_def"
 
 val Ev_def = Exp_def |> spec_all |> rewr_rule[isExp_def]
                      |> ex2fsym0 "Ev" ["A","B"]
+                     |> store_as "Ev_def"
 
 val Tp_def = Ev_def |> spec_all |> uex_expand 
                     |> ex2fsym0 "Tp" ["f"]
+                    |> store_as "Tp_def"
 
 
-val N_ex = new_ax “?N O:1->N SUC:N->N.
- !X x0:1->X t:X->X.?!x:N->X. x o O = x0 & x o SUC = t o x”
+val N_ex = store_ax("N_ex",“?N O:1->N SUC:N->N.
+ !X x0:1->X t:X->X.?!x:N->X. x o O = x0 & x o SUC = t o x”)
 
-val N_def = N_ex |> ex2fsym0 "N" []
+val N_def = N_ex |> ex2fsym0 "N" [] |> store_as "N_def";
 
-val O_def = N_def |> ex2fsym0 "O" []
+val O_def = N_def |> ex2fsym0 "O" [] |> store_as "O_def";
 
-val SUC_def = O_def |> ex2fsym0 "SUC" []
+val SUC_def = O_def |> ex2fsym0 "SUC" [] |> store_as "SUC_def";
 
-val WP = new_ax “!A B f:A->B g.~(f = g) ==> ?a:1->A. ~(f o a = g o a)”
+val WP = store_ax("WP",“!A B f:A->B g.~(f = g) ==> ?a:1->A. ~(f o a = g o a)”);
 
 
 (*mono does not need "is" version becuase it does not induce any function*)
 val _ = new_pred "Mono" [("f",ar_sort (mk_ob "A") (mk_ob "B"))]
 
-val Mono_def = new_ax “!A B f:A->B. Mono(f) <=> !X g:X->A h. f o g = f o h ==> g = h”
+val Mono_def = store_ax("Mono_def",“!A B f:A->B. Mono(f) <=> !X g:X->A h. f o g = f o h ==> g = h”);
 
-val NONZERO_EL = new_ax “!X.~(is0(X)) ==>?x:1->X.T”
+val NONZERO_EL = store_ax("NONZERO_EL",“!X.~(is0(X)) ==>?x:1->X.T”);
 
-val AC = new_ax “!A B f:A->B. ?g:B->A. f o g o f = f”;
+val AC = store_ax("AC",“!A B f:A->B. ?g:B->A. f o g o f = f”);
 
+val INC_FAC = store_ax("INC_FAC",“!A B f:1->A + B. (?f0:1->A.i1(A,B) o f0 = f) |(?f0:1->B.i2(A,B) o f0 = f)”);
 
-val ismem_def = read_axiom "!A x:1-> A A0 a:A0 -> A. ismem(x,a) <=> ismono(a) & ?x0:1 -> A0. a o x0 = x";
+val DISTI_EL = store_ax("DISTI_EL",“?X x1:1->X x2. ~(x1 = x2)”)
 
-val INC_FAC = new_ax “!A B f:1->A + B. (?f0:1->A.i1(A,B) o f0 = f) |(?f0:1->B.i2(A,B) o f0 = f)”
+val FALSE_ex = prove_store ("FALSE_ex",
+e0
+(qexists_tac ‘i1(1,1)’ >> rw[])
+(form_goal
+ “?f. i1(1,1) = f”)
+)
 
-val DISTI_EL = new_ax “?X x1:1->X x2. ~(x1 = x2)”
+val FALSE_def = ex2fsym0 "FALSE" [] FALSE_ex 
+                         |> store_as "FALSE_def"
+
+val TRUE_ex = prove_store ("TRUE_ex",
+e0
+(qexists_tac ‘i2(1,1)’ >> rw[])
+(form_goal
+ “?f. i2(1,1) = f”)
+)
+
+val TRUE_def = ex2fsym0 "TRUE" [] FALSE_ex 
+                        |> store_as "TRUE_def"
 
